Mbse.lean
@@ -4,6 +4,7 @@ import Mbse.Wymore
 import Mbse.Notation
 import Mbse.CombinationalWymore
 import Mbse.DPDAWymore
+import Mbse.DPDAExamples
 import Mbse.GeneralizedWymore
 
 
